Hoare/Hoare_Step.thy
@@ -445,6 +445,13 @@ proof(rule HT'I)
         have Dominate1 : "pcomps fs_sub x m = f' x m"
           using dominant_pcomps[OF Pres'[unfolded sym[OF Fs_sub]] Hnemp[unfolded sym[OF Fs_sub]] Hdom' Xin Ok]
           by auto
+(*
+        (* Can we weaken our definition of dominant? *)
+        have Dominate1_weak :
+          "LOut (no_control_lifting l) (l' x) (pcomps fs_sub x m) =
+           LOut (no_control_lifting l) (l' x) (f' x m)"
+          sorry
+*)
 
 (* YOU ARE HERE. *)
 (* problem: seems like we still need to know something about the validity of the initial state.
@@ -454,7 +461,7 @@ proof(rule HT'I)
  *)
         obtain pri1 pri2 rest where Msplit :
           "m = (mdp pri1 (Some (mdt (G x z # c'))), mdp pri2 (Some (mdt (STR ''''))), rest)" and Rest : "rest \<in> ok_S"
-          using Gs_alt' Dominate1 Skip Hpay Hcont Hf' Hpay_S
+          using Gs_alt' Dominate1 (*Dominate1_weak*) Skip Hpay Hcont Hf' Hpay_S
           by(auto simp add: seq_sem_l_gen_def seq_sem_lifting_gen_def 
             lift_pred_valid_ok_s_def lift_pred_noS_s_def lift_pred_s_def lift_map_s_def
             no_control_lifting_def cont_def
