Mergeable/Bump.thy
@@ -1,0 +1,18 @@
+theory Bump
+  imports Mergeable
+begin
+
+(* Captures an important extension of mergeable - 
+ * situations where we are dealing with a type (such as md_prio)
+ * where we can easily calculate, for any valid x, the "next
+ * largest value with the same contents
+ *)
+
+(* This is most useful when used with liftings; see the Lifter directory for details. *)
+
+class Bump = Pord_Weak +
+  fixes bump :: "'a \<Rightarrow> 'a"
+  assumes bump_neq : "\<And> x . bump x \<noteq> x"
+  assumes bump_geq : "\<And> x . x <[ bump x"
+
+end
